FactoryGameStuff.v
@@ -9,16 +9,16 @@ Import EqNotations.
 Require Import Coq.Program.Equality.
 Load EliUtils.
 (* Require Import Eli.EliUtils.
-
-Locate "<". *)
+ *)
 
 Notation "a ∈ c" := (In a c) (at level 60, no associativity) : type_scope.
 Notation "a ∉ c" := (¬In a c) (at level 60, no associativity) : type_scope.
+Notation "g [ i ]" := (Vector.nth g i) (at level 60, no associativity) : type_scope.
 
 Definition Graph n := Vector.t (list (Fin.t n)) n.
 
 Definition HasPredecessorLeft n (graph : Graph n) (partial_result : list (Fin.t n)) (node : Fin.t n) :=
-  ∃ (predecessor : Fin.t n) (edge : listIndex (Vector.nth graph predecessor)), predecessor ∉ partial_result ∧ valueAt edge = node.
+  ∃ (predecessor : Fin.t n) (edge : listIndex (graph[predecessor])), predecessor ∉ partial_result ∧ valueAt edge = node.
   
 Inductive TopoStep n (graph : Graph n) (partial_result : list (Fin.t n)) :=
 | TopoStepDone (_: ∀ node, HasPredecessorLeft graph partial_result node)
@@ -26,21 +26,108 @@ Inductive TopoStep n (graph : Graph n) (partial_result : list (Fin.t n)) :=
 
 Inductive PartialTopoSort n (graph : Graph n) : list (Fin.t n) → Prop :=
 | TopoSortNil : PartialTopoSort graph nil
-| TopoSortCons partial_result next (_: ¬HasPredecessorLeft graph partial_result next) : PartialTopoSort graph (next :: partial_result).
+| TopoSortCons partial_result next : ¬In next partial_result → ¬HasPredecessorLeft graph partial_result next → PartialTopoSort graph (partial_result) → PartialTopoSort graph (next :: partial_result).
 
 Definition TopoSort n (graph : Graph n) (partial_result : list (Fin.t n)) : Prop := PartialTopoSort graph partial_result ∧ ∀ node, HasPredecessorLeft graph partial_result node.
+
+
+Lemma PartialTopoSort_NotIn_IfEdgeTo 
+  n (graph : Graph n) partial_result (sort : PartialTopoSort graph partial_result)
+  (node : Fin.t n) (edge : listIndex (graph[node]))
+  : node ∉ partial_result → (valueAt edge) ∉ partial_result.
+  intuition idtac; dependent induction sort. easy.
+  specialize (IHsort node edge (λ tail, H1 (or_intror tail))).
+  destruct (eq_dec next (valueAt edge)).
+  rewrite e in *. contradict H0. exists node; exists edge; split.
+  contradict H1; right; assumption. reflexivity.
+  destruct H2; contradiction.
+Qed.
 
 Lemma PartialTopoSort_is_topological
   n (graph : Graph n) partial_result (sort : PartialTopoSort graph partial_result)
   : 
   (* "If there's an edge from i0 to i1, i1 must come first" *)
-  ∀ (i0 i1 : listIndex partial_result) (edge : listIndex (Vector.nth graph (valueAt i0))),
+  ∀ (i0 i1 : listIndex partial_result) (edge : listIndex (graph[valueAt i0])),
     valueAt edge = valueAt i1 →
     positionOf i1 < positionOf i0.
+  
+  intros; dependent induction sort. easy.
+  
+  dependent destruction i1; dependent destruction i0; cbn in *.
+  
+  contradict H0; exists next; exists edge; tauto.
+  apply PeanoNat.Nat.lt_0_succ.
+  exfalso. pose (PartialTopoSort_NotIn_IfEdgeTo sort next edge H) as vnp. rewrite H1 in *. exact (vnp (listIndex_In i1)).
+  
+  apply Lt.lt_n_S. exact (IHsort i0 i1 edge H1).
+Qed.
+  
+Search "fold".
+Definition InEdgeCount_one n (edges : list (Fin.t n)) i := fold_left (λ count edge, if eq_dec edge i then S count else count) edges 0.
+Definition InEdgeCount n (graph : Graph n) partial_result i := Vector.fold_left (λ count edges, if in_dec eq_dec i partial_result then count else count + InEdgeCount_one edges i) 0 graph.
+Definition InEdgeCounts n (graph : Graph n) (counts : Vector.t nat n) partial_result := ∀ i, counts[i] = InEdgeCount graph partial_result i.
+
+Record TopoSortAlgo_State n := mkTopoSortAlgo_State
+  { in_edge_counts : Vector.t nat n
+  ; unrecorded_nodes_with_no_in_edges : list (Fin.t n)
+  ; partial_result : list (Fin.t n)
+  }.
+  
+Definition TopoSortAlgo_State_Valid n (graph : Graph n) state :=
+  InEdgeCounts graph (in_edge_counts state) (partial_result state) ∧ (∀ i, (in_edge_counts state)[i] = 0 ↔ i ∈ unrecorded_nodes_with_no_in_edges state) ∧ NoDup (unrecorded_nodes_with_no_in_edges state) ∧ PartialTopoSort graph (partial_result state).
+
+Fixpoint uncount_edges
+  n (graph : Graph n) 
+  (in_edge_counts : Vector.t nat n)
+  (unrecorded_nodes_with_no_in_edges : list (Fin.t n))
+  (dsts : list (Fin.t n))
+  : Vector.t nat n × list (Fin.t n)
+  := match dsts with
+  | nil => (in_edge_counts, unrecorded_nodes_with_no_in_edges)
+  | dst :: tail => let (in_edge_counts, unrecorded_nodes_with_no_in_edges) := uncount_edges graph in_edge_counts unrecorded_nodes_with_no_in_edges tail in
+    let new := in_edge_counts[dst] - 1 in (
+    Vector.replace in_edge_counts dst new,
+    match new with
+    | 0 => dst :: unrecorded_nodes_with_no_in_edges
+    | S _ => unrecorded_nodes_with_no_in_edges
+    end)
+  end.
+  
+
+Definition TopoSortAlgo_step
+  n (graph : Graph n)
+  (state : TopoSortAlgo_State n)
+  : TopoSortAlgo_State n + list (Fin.t n)
+  := 
+  match unrecorded_nodes_with_no_in_edges state with
+  | nil => inr (partial_result state)
+  | head :: tail => let (in_edge_counts, unrecorded_nodes_with_no_in_edges) := (uncount_edges graph (in_edge_counts state) tail (graph[head])) in
+  inl (mkTopoSortAlgo_State
+    in_edge_counts
+    unrecorded_nodes_with_no_in_edges
+    (head :: partial_result state)
+  )
+  end.
+
+Lemma TopoSortAlgo_step_valid
+  n (graph : Graph n)
+  (state : TopoSortAlgo_State n)
+  (state_valid : TopoSortAlgo_State_Valid graph state)
+  (step_result := TopoSortAlgo_step graph state)
+  : match step_result with
+    | inr result => TopoSort graph result
+    | inl state => TopoSortAlgo_State_Valid graph state
+    end.
+  destruct state.
+  destruct state_valid as [counts_valid q]; destruct q as [unrecorded_correct q]; destruct q as [unrecorded_nodup partial_sort].
+  destruct unrecorded_nodes_with_no_in_edges0; cbn in *.
+  
+  split.
+  assumption.
+  intros.
+  
   admit.
-Admitted.  
-
-
+  
 (*
   
 Definition graphRemove n
